theories/mlanguage/lifting.v
@@ -18,13 +18,15 @@ Implicit Types X : expr Λ * state Λ → Prop.
 
 Lemma wp_lift_step_fupd pe E Φ e1 :
   to_val e1 = None → 
+  not_is_ext_call (penv_prog pe) e1 →
   (∀ σ1, state_interp σ1 ={E}=∗
     ∀ X, ⌜prim_step (penv_prog pe) (e1, σ1) X⌝ ={E}▷=∗^(1) |={E}=>
       ∃ e2 σ2,
         ⌜X (e2, σ2)⌝ ∗ state_interp σ2 ∗ WP e2 @ pe; E {{ Φ }})
   ⊢ WP e1 @ pe; E {{ Φ }}.
-Proof. intros H. rewrite wp_unfold /wp_pre.
+Proof. intros Hval Hcall. rewrite wp_unfold /wp_pre.
   iIntros "H %σ Hσ". iMod ("H" $! σ with "Hσ") as "H2". iModIntro. do 2 iRight.
+  iSplitR; first done.
   iSplitR; first done.
   iIntros (X Hstep). iMod ("H2" $! X Hstep) as "H2". do 2 iModIntro.
   do 2 iMod "H2". iModIntro. iFrame.
@@ -36,13 +38,14 @@ Qed.
 
 Lemma wp_lift_atomic_step {pe E Φ} e1 :
   to_val e1 = None →
+  not_is_ext_call (penv_prog pe) e1 →
   (∀ σ1, state_interp σ1 ={E}=∗
     ▷ ∀ X, ⌜prim_step (penv_prog pe) (e1, σ1) X⌝ ={E}=∗
       ∃ e2 σ2, ⌜X (e2, σ2)⌝ ∗
         state_interp σ2 ∗ from_option Φ False (to_val e2))
   ⊢ WP e1 @ pe; E {{ Φ }}.
 Proof.
-  iIntros (?) "H".
+  iIntros (Hnv Hnc) "H".
   iApply (wp_lift_step_fupd pe E _ e1)=>//; iIntros (σ1) "Hσ1".
   iMod ("H" $! σ1 with "Hσ1") as "H". iModIntro.
   iIntros (X Hstep). do 3 iModIntro.
@@ -54,13 +57,14 @@ Qed.
 
 Lemma wp_lift_atomic_prim_step {pe E Φ} e1 :
   to_val e1 = None →
+  not_is_ext_call (penv_prog pe) e1 →
   (∀ σ1, state_interp σ1 ={E}=∗
     ▷ ∀ X, ⌜prim_step (penv_prog pe) (e1, σ1) X⌝ ={E}=∗
       ∃ e2 σ2, ⌜X (e2, σ2)⌝ ∗
         state_interp σ2 ∗ from_option Φ False (to_val e2))
   ⊢ WP e1 @ pe; E {{ Φ }}.
 Proof.
-  iIntros (?) "H".
+  iIntros (Hnv Hnc) "H".
   iApply (wp_lift_step_fupd pe E _ e1)=>//; iIntros (σ1) "Hσ1".
   iMod ("H" $! σ1 with "Hσ1") as "H". iModIntro.
   iIntros (X Hstep).
@@ -78,6 +82,9 @@ Lemma wp_lift_pure_det_step `{!Inhabited (state Λ)} {pe E Φ} e1 e2 :
   (|={E}[E]▷=> WP e2 @ pe; E {{ Φ }}) ⊢ WP e1 @ pe; E {{ Φ }}.
 Proof.
   iIntros (Hsafe Hstep) "H". iApply wp_lift_step_fupd; first done.
+  { intros (f&vs&C&H1&H2). eapply (Hstep inhabitant (λ _, False)).
+    eapply call_prim_step; first done.
+    intros ? ? ?; congruence. }
   iIntros (σ1) "Hσ". iMod "H". iModIntro.
   iIntros (X Hstep'). do 3 iModIntro. iMod "H".
   iModIntro. iExists e2, _. iSplitR.
